Revert "Optimize dettman algorithm"

fiat-amd64/fiat_secp256k1_dettman_mul/seed0000000218287519_ratio10697.asm
@@ -1,0 +1,212 @@
+SECTION .text
+	GLOBAL fiat_secp256k1_dettman_mul
+fiat_secp256k1_dettman_mul:
+mov rax, rdx
+mov rdx, [ rsi + 0x10 ]
+mulx r11, r10, [ rax + 0x8 ]
+mov rdx, [ rsi + 0x20 ]
+mulx r8, rcx, [ rax + 0x20 ]
+mov rdx, [ rsi + 0x20 ]
+mov [ rsp - 0x80 ], rbx
+mulx rbx, r9, [ rax + 0x18 ]
+mov rdx, [ rax + 0x20 ]
+mov [ rsp - 0x78 ], rbp
+mov [ rsp - 0x70 ], r12
+mulx r12, rbp, [ rsi + 0x0 ]
+mov rdx, [ rsi + 0x0 ]
+mov [ rsp - 0x68 ], r13
+mov [ rsp - 0x60 ], r14
+mulx r14, r13, [ rax + 0x18 ]
+mov rdx, [ rax + 0x10 ]
+mov [ rsp - 0x58 ], r15
+mov [ rsp - 0x50 ], rdi
+mulx rdi, r15, [ rsi + 0x8 ]
+mov rdx, [ rsi + 0x18 ]
+mov [ rsp - 0x48 ], rbx
+mov [ rsp - 0x40 ], r9
+mulx r9, rbx, [ rax + 0x20 ]
+mov rdx, 0xfffffffffffff 
+mov [ rsp - 0x38 ], r9
+mov r9, rcx
+and r9, rdx
+mov rdx, [ rax + 0x0 ]
+mov [ rsp - 0x30 ], rbx
+mov [ rsp - 0x28 ], r12
+mulx r12, rbx, [ rsi + 0x18 ]
+adox rbx, r10
+adox r11, r12
+adcx rbx, r15
+adcx rdi, r11
+test al, al
+adox rbx, r13
+adox r14, rdi
+shrd rcx, r8, 52
+mov rdx, [ rsi + 0x20 ]
+mulx r8, r10, [ rax + 0x0 ]
+mov rdx, [ rsi + 0x18 ]
+mulx r15, r13, [ rax + 0x8 ]
+add r10, r13
+adcx r15, r8
+mov rdx, [ rsi + 0x10 ]
+mulx r11, r12, [ rax + 0x10 ]
+mov rdx, 0x1000003d10 
+mulx r8, rdi, r9
+mulx r13, r9, rcx
+add rdi, rbx
+adcx r14, r8
+add r10, r12
+adcx r11, r15
+mov rdx, [ rsi + 0x8 ]
+mulx rcx, rbx, [ rax + 0x18 ]
+test al, al
+adox r10, rbx
+adox rcx, r11
+mov rdx, 0x34 
+bzhi r15, rdi, rdx
+mov rdx, [ rax + 0x8 ]
+mulx r8, r12, [ rsi + 0x20 ]
+mov rdx, [ rax + 0x10 ]
+mulx rbx, r11, [ rsi + 0x18 ]
+adox r12, r11
+adox rbx, r8
+mov rdx, [ rsi + 0x10 ]
+mulx r11, r8, [ rax + 0x18 ]
+test al, al
+adox r12, r8
+adox r11, rbx
+shrd rdi, r14, 52
+xor rdx, rdx
+adox r10, rbp
+adox rcx, [ rsp - 0x28 ]
+adcx rdi, r10
+adc rcx, 0x0
+mov rdx, [ rax + 0x20 ]
+mulx r14, rbp, [ rsi + 0x8 ]
+xor rdx, rdx
+adox r9, rdi
+adox rcx, r13
+mov r13, r9
+shrd r13, rcx, 52
+xor rbx, rbx
+adox r12, rbp
+adox r14, r11
+adcx r13, r12
+adc r14, 0x0
+mov rdx, r13
+shrd rdx, r14, 52
+mov r8, 0x34 
+bzhi r11, r13, r8
+bzhi r10, r9, r8
+mov rdi, r10
+shr rdi, 48
+mov rbp, rdx
+mov rdx, [ rsi + 0x18 ]
+mulx rcx, r9, [ rax + 0x18 ]
+shl r11, 4
+lea r11, [ r11 + rdi ]
+mov rdx, 0x1000003d1 
+mulx r13, r12, r11
+mov rdx, [ rsi + 0x0 ]
+mulx rdi, r14, [ rax + 0x0 ]
+test al, al
+adox r12, r14
+adox rdi, r13
+mov rdx, [ rsi + 0x20 ]
+mulx r13, r11, [ rax + 0x10 ]
+adcx r11, r9
+adcx rcx, r13
+mov rdx, [ rsi + 0x10 ]
+mulx r14, r9, [ rax + 0x20 ]
+xor rdx, rdx
+adox r11, r9
+adox r14, rcx
+bzhi rbx, r12, r8
+shrd r12, rdi, 52
+xor rdi, rdi
+adox rbp, r11
+adox r14, rdi
+mov rdx, [ rsp - 0x50 ]
+mov [ rdx + 0x0 ], rbx
+bzhi r13, rbp, r8
+mov rcx, [ rsp - 0x30 ]
+mov r9, rcx
+adox r9, [ rsp - 0x40 ]
+mov r11, [ rsp - 0x38 ]
+adox r11, [ rsp - 0x48 ]
+mov rcx, rdx
+mov rdx, [ rsi + 0x0 ]
+mulx rdi, rbx, [ rax + 0x8 ]
+shrd rbp, r14, 52
+xor rdx, rdx
+adox rbp, r9
+adox r11, rdx
+bzhi r14, rbp, r8
+shrd rbp, r11, 52
+mov rdx, [ rax + 0x0 ]
+mulx r11, r9, [ rsi + 0x8 ]
+test al, al
+adox r9, rbx
+adox rdi, r11
+mov rdx, 0x1000003d10 
+mulx r11, rbx, r13
+adcx r12, r9
+adc rdi, 0x0
+xor r13, r13
+adox rbx, r12
+adox rdi, r11
+mov rdx, [ rsi + 0x0 ]
+mulx r11, r9, [ rax + 0x10 ]
+mov rdx, [ rax + 0x0 ]
+mulx r13, r12, [ rsi + 0x10 ]
+mov rdx, [ rsi + 0x8 ]
+mulx rcx, r8, [ rax + 0x8 ]
+adcx r12, r8
+adcx rcx, r13
+xor rdx, rdx
+adox r12, r9
+adox r11, rcx
+mov r9, rbx
+shrd r9, rdi, 52
+xor rdi, rdi
+adox r9, r12
+adox r11, rdi
+mov rdx, 0x1000003d10 
+mulx r8, r13, r14
+adcx r13, r9
+adcx r11, r8
+mov r14, 0x34 
+bzhi rcx, r13, r14
+mulx r9, r12, rbp
+shrd r13, r11, 52
+lea r15, [ r15 + r13 ]
+add r12, r15
+adc r9, 0x0
+bzhi rbp, rbx, r14
+bzhi rbx, r12, r14
+mov r8, [ rsp - 0x50 ]
+mov [ r8 + 0x18 ], rbx
+mov r11, 0x30 
+bzhi r13, r10, r11
+shrd r12, r9, 52
+lea r13, [ r13 + r12 ]
+mov [ r8 + 0x20 ], r13
+mov [ r8 + 0x8 ], rbp
+mov [ r8 + 0x10 ], rcx
+mov rbx, [ rsp - 0x80 ]
+mov rbp, [ rsp - 0x78 ]
+mov r12, [ rsp - 0x70 ]
+mov r13, [ rsp - 0x68 ]
+mov r14, [ rsp - 0x60 ]
+mov r15, [ rsp - 0x58 ]
+ret
+; cpu Intel(R) Core(TM) i7-6770HQ CPU @ 2.60GHz
+; ratio 1.0697
+; seed 0757023763997057 
+; CC / CFLAGS clang / -march=native -mtune=native -O3 
+; time needed: 2179788 ms on 180000 evaluations.
+; Time spent for assembling and measuring (initial batch_size=152, initial num_batches=31): 140036 ms
+; number of used evaluations: 180000
+; Ratio (time for assembling + measure)/(total runtime for 180000 evals): 0.06424294472673489
+; number reverted permutation / tried permutation: 71202 / 90172 =78.962%
+; number reverted decision / tried decision: 52572 / 89827 =58.526%
+; validated in 0.593s
