fiat-amd64/fiat_secp256k1_dettman_mul/seed0000000451748095_ratio12970.asm
@@ -1,0 +1,209 @@
+SECTION .text
+	GLOBAL fiat_secp256k1_dettman_mul
+fiat_secp256k1_dettman_mul:
+mov rax, rdx
+mov rdx, [ rsi + 0x10 ]
+mulx r11, r10, [ rax + 0x8 ]
+mov rdx, [ rax + 0x10 ]
+mulx r8, rcx, [ rsi + 0x8 ]
+mov rdx, [ rax + 0x20 ]
+mov [ rsp - 0x80 ], rbx
+mulx rbx, r9, [ rsi + 0x20 ]
+mov rdx, [ rax + 0x0 ]
+mov [ rsp - 0x78 ], rbp
+mov [ rsp - 0x70 ], r12
+mulx r12, rbp, [ rsi + 0x18 ]
+xor rdx, rdx
+adox rbp, r10
+adox r11, r12
+mov rdx, [ rax + 0x18 ]
+mulx r12, r10, [ rsi + 0x8 ]
+adcx rbp, rcx
+adcx r8, r11
+mov rdx, [ rax + 0x18 ]
+mulx r11, rcx, [ rsi + 0x0 ]
+add rbp, rcx
+adcx r11, r8
+mov rdx, [ rsi + 0x18 ]
+mulx rcx, r8, [ rax + 0x8 ]
+mov rdx, 0xfffffffffffff 
+mov [ rsp - 0x68 ], r13
+mov r13, r9
+and r13, rdx
+mov rdx, [ rax + 0x0 ]
+mov [ rsp - 0x60 ], r14
+mov [ rsp - 0x58 ], r15
+mulx r15, r14, [ rsi + 0x20 ]
+mov rdx, 0x1000003d10 
+mov [ rsp - 0x50 ], rdi
+mov [ rsp - 0x48 ], r12
+mulx r12, rdi, r13
+adox rdi, rbp
+adox r11, r12
+mov rbp, rdi
+shrd rbp, r11, 52
+add r14, r8
+adcx rcx, r15
+mov rdx, [ rax + 0x10 ]
+mulx r13, r8, [ rsi + 0x10 ]
+mov rdx, [ rsi + 0x0 ]
+mulx r12, r15, [ rax + 0x20 ]
+test al, al
+adox r14, r8
+adox r13, rcx
+adcx r14, r10
+adcx r13, [ rsp - 0x48 ]
+test al, al
+adox r14, r15
+adox r12, r13
+adcx rbp, r14
+adc r12, 0x0
+shrd r9, rbx, 52
+mov rdx, 0x1000003d10 
+mulx r10, rbx, r9
+add rbx, rbp
+adcx r12, r10
+mov r11, rbx
+shrd r11, r12, 52
+mov rdx, [ rsi + 0x18 ]
+mulx r8, rcx, [ rax + 0x10 ]
+mov rdx, [ rsi + 0x8 ]
+mulx r13, r15, [ rax + 0x20 ]
+mov rdx, [ rax + 0x8 ]
+mulx rbp, r14, [ rsi + 0x20 ]
+test al, al
+adox r14, rcx
+adox r8, rbp
+mov rdx, [ rax + 0x18 ]
+mulx r10, r9, [ rsi + 0x10 ]
+adcx r14, r9
+adcx r10, r8
+add r14, r15
+adcx r13, r10
+mov rdx, [ rax + 0x18 ]
+mulx rcx, r12, [ rsi + 0x18 ]
+xor rdx, rdx
+adox r11, r14
+adox r13, rdx
+mov r15, 0xfffffffffffff 
+mov rbp, r11
+and rbp, r15
+mov rdx, [ rax + 0x10 ]
+mulx r9, r8, [ rsi + 0x20 ]
+shl rbp, 4
+and rbx, r15
+adox r8, r12
+adox rcx, r9
+mov rdx, 0xffffffffffff 
+mov r10, rbx
+and r10, rdx
+mov rdx, [ rsi + 0x10 ]
+mulx r12, r14, [ rax + 0x20 ]
+shr rbx, 48
+lea rbp, [ rbp + rbx ]
+mov rdx, 0x1000003d1 
+mulx rbx, r9, rbp
+mov rdx, [ rax + 0x8 ]
+mulx r15, rbp, [ rsi + 0x0 ]
+mov rdx, [ rsi + 0x0 ]
+mov [ rsp - 0x40 ], r10
+mov [ rsp - 0x38 ], r15
+mulx r15, r10, [ rax + 0x0 ]
+shrd r11, r13, 52
+test al, al
+adox r8, r14
+adox r12, rcx
+adcx r11, r8
+adc r12, 0x0
+mov rdx, r11
+shrd rdx, r12, 52
+add r9, r10
+adcx r15, rbx
+mov r13, r9
+shrd r13, r15, 52
+mov rcx, 0xfffffffffffff 
+and r11, rcx
+mov r14, rdx
+mov rdx, [ rax + 0x18 ]
+mulx r10, rbx, [ rsi + 0x20 ]
+mov rdx, [ rsi + 0x18 ]
+mulx r12, r8, [ rax + 0x20 ]
+adox rbx, r8
+adox r12, r10
+adcx r14, rbx
+adc r12, 0x0
+mov rdx, [ rsi + 0x8 ]
+mulx r10, r15, [ rax + 0x0 ]
+mov rdx, 0x1000003d10 
+mulx rbx, r8, r11
+mov r11, r14
+shrd r11, r12, 52
+xor r12, r12
+adox r15, rbp
+adox r10, [ rsp - 0x38 ]
+adcx r13, r15
+adc r10, 0x0
+add r8, r13
+adcx r10, rbx
+mov rdx, [ rax + 0x0 ]
+mulx rbx, rbp, [ rsi + 0x10 ]
+mov rdx, [ rsi + 0x8 ]
+mulx r13, r15, [ rax + 0x8 ]
+mov rdx, [ rax + 0x10 ]
+mulx rcx, r12, [ rsi + 0x0 ]
+xor rdx, rdx
+adox rbp, r15
+adox r13, rbx
+mov rbx, r8
+shrd rbx, r10, 52
+test al, al
+adox rbp, r12
+adox rcx, r13
+adcx rbx, rbp
+adc rcx, 0x0
+mov r10, 0xfffffffffffff 
+and r14, r10
+mov r15, 0x1000003d10 
+mov rdx, r15
+mulx r12, r15, r14
+adox r15, rbx
+adox rcx, r12
+mov r13, r15
+shrd r13, rcx, 52
+and r15, r10
+and rdi, r10
+lea rdi, [ rdi + r13 ]
+mov rbp, [ rsp - 0x50 ]
+mov [ rbp + 0x10 ], r15
+mulx r14, rbx, r11
+adox rbx, rdi
+mov r11, 0x0 
+adox r14, r11
+mov r12, rbx
+shrd r12, r14, 52
+add r12, [ rsp - 0x40 ]
+and r9, r10
+mov [ rbp + 0x0 ], r9
+and r8, r10
+and rbx, r10
+mov [ rbp + 0x8 ], r8
+mov [ rbp + 0x20 ], r12
+mov [ rbp + 0x18 ], rbx
+mov rbx, [ rsp - 0x80 ]
+mov rbp, [ rsp - 0x78 ]
+mov r12, [ rsp - 0x70 ]
+mov r13, [ rsp - 0x68 ]
+mov r14, [ rsp - 0x60 ]
+mov r15, [ rsp - 0x58 ]
+ret
+; cpu 13th Gen Intel(R) Core(TM) i9-13900KF
+; ratio 1.2970
+; seed 1264522544272874 
+; CC / CFLAGS clang / -march=native -mtune=native -O3 
+; time needed: 837498 ms on 180000 evaluations.
+; Time spent for assembling and measuring (initial batch_size=325, initial num_batches=31): 80113 ms
+; number of used evaluations: 180000
+; Ratio (time for assembling + measure)/(total runtime for 180000 evals): 0.0956575418687567
+; number reverted permutation / tried permutation: 73615 / 89948 =81.842%
+; number reverted decision / tried decision: 53670 / 90051 =59.600%
+; validated in 0.248s
