fiat-amd64/fiat_secp256k1_dettman_mul/seed0000000843851796_ratio10725.asm
@@ -1,0 +1,216 @@
+SECTION .text
+	GLOBAL fiat_secp256k1_dettman_mul
+fiat_secp256k1_dettman_mul:
+mov rax, rdx
+mov rdx, [ rdx + 0x10 ]
+mulx r11, r10, [ rsi + 0x18 ]
+mov rdx, [ rsi + 0x0 ]
+mulx r8, rcx, [ rax + 0x8 ]
+mov rdx, [ rsi + 0x8 ]
+mov [ rsp - 0x80 ], rbx
+mulx rbx, r9, [ rax + 0x18 ]
+mov rdx, [ rsi + 0x18 ]
+mov [ rsp - 0x78 ], rbp
+mov [ rsp - 0x70 ], r12
+mulx r12, rbp, [ rax + 0x0 ]
+mov rdx, [ rax + 0x0 ]
+mov [ rsp - 0x68 ], r13
+mov [ rsp - 0x60 ], r14
+mulx r14, r13, [ rsi + 0x10 ]
+mov rdx, [ rsi + 0x20 ]
+mov [ rsp - 0x58 ], r15
+mov [ rsp - 0x50 ], rdi
+mulx rdi, r15, [ rax + 0x8 ]
+add r15, r10
+adcx r11, rdi
+mov rdx, [ rsi + 0x10 ]
+mulx rdi, r10, [ rax + 0x18 ]
+mov rdx, [ rax + 0x10 ]
+mov [ rsp - 0x48 ], r14
+mov [ rsp - 0x40 ], r13
+mulx r13, r14, [ rsi + 0x0 ]
+mov rdx, [ rsi + 0x20 ]
+mov [ rsp - 0x38 ], r13
+mov [ rsp - 0x30 ], r14
+mulx r14, r13, [ rax + 0x0 ]
+mov rdx, [ rax + 0x8 ]
+mov [ rsp - 0x28 ], r8
+mov [ rsp - 0x20 ], rcx
+mulx rcx, r8, [ rsi + 0x18 ]
+xor rdx, rdx
+adox r13, r8
+adox rcx, r14
+mov rdx, [ rsi + 0x10 ]
+mulx r8, r14, [ rax + 0x10 ]
+adcx r15, r10
+adcx rdi, r11
+mov rdx, [ rsi + 0x20 ]
+mulx r10, r11, [ rax + 0x10 ]
+add r13, r14
+adcx r8, rcx
+mov rdx, [ rsi + 0x18 ]
+mulx r14, rcx, [ rax + 0x18 ]
+test al, al
+adox r13, r9
+adox rbx, r8
+adcx r11, rcx
+adcx r14, r10
+mov rdx, [ rsi + 0x20 ]
+mulx r10, r9, [ rax + 0x20 ]
+mov rdx, [ rsi + 0x8 ]
+mulx rcx, r8, [ rax + 0x10 ]
+mov rdx, [ rax + 0x8 ]
+mov [ rsp - 0x18 ], r14
+mov [ rsp - 0x10 ], r11
+mulx r11, r14, [ rsi + 0x10 ]
+add rbp, r14
+adcx r11, r12
+xor rdx, rdx
+adox rbp, r8
+adox rcx, r11
+mov r12, 0xfffffffffffff 
+mov r8, r9
+and r8, r12
+mov rdx, [ rax + 0x18 ]
+mulx r11, r14, [ rsi + 0x0 ]
+mov rdx, 0x1000003d10 
+mov [ rsp - 0x8 ], rdi
+mulx rdi, r12, r8
+adox rbp, r14
+adox r11, rcx
+adcx r12, rbp
+adcx r11, rdi
+mov rcx, r12
+shrd rcx, r11, 52
+mov rdx, [ rax + 0x20 ]
+mulx r14, r8, [ rsi + 0x0 ]
+xor rdx, rdx
+adox r13, r8
+adox r14, rbx
+shrd r9, r10, 52
+add rcx, r13
+adc r14, 0x0
+mov rbx, 0x1000003d10 
+mov rdx, rbx
+mulx r10, rbx, r9
+test al, al
+adox rbx, rcx
+adox r14, r10
+mov rdi, 0xfffffffffffff 
+and r12, rdi
+mov rbp, rbx
+shrd rbp, r14, 52
+mov rdx, [ rsi + 0x8 ]
+mulx r8, r11, [ rax + 0x20 ]
+and rbx, rdi
+adox r15, r11
+adox r8, [ rsp - 0x8 ]
+mov rdx, 0xffffffffffff 
+mov r13, rbx
+and r13, rdx
+shr rbx, 48
+add rbp, r15
+adc r8, 0x0
+mov r9, rbp
+and r9, rdi
+shrd rbp, r8, 52
+mov rdx, [ rax + 0x20 ]
+mulx r10, rcx, [ rsi + 0x10 ]
+shl r9, 4
+lea r9, [ r9 + rbx ]
+mov rdx, rcx
+add rdx, [ rsp - 0x10 ]
+adcx r10, [ rsp - 0x18 ]
+mov r14, rdx
+mov rdx, [ rax + 0x20 ]
+mulx r15, r11, [ rsi + 0x18 ]
+mov rdx, 0x1000003d1 
+mulx r8, rbx, r9
+mov rdx, [ rsi + 0x0 ]
+mulx r9, rcx, [ rax + 0x0 ]
+xor rdx, rdx
+adox rbp, r14
+adox r10, rdx
+mov rdx, [ rax + 0x18 ]
+mulx rdi, r14, [ rsi + 0x20 ]
+adcx r14, r11
+adcx r15, rdi
+mov rdx, 0x34 
+bzhi r11, rbp, rdx
+adox rbx, rcx
+adox r9, r8
+shrd rbp, r10, 52
+bzhi r8, rbx, rdx
+adox rbp, r14
+mov rcx, 0x0 
+adox r15, rcx
+mov rdx, [ rsi + 0x8 ]
+mulx rdi, r10, [ rax + 0x0 ]
+mov rdx, 0x1000003d10 
+mulx rcx, r14, r11
+test al, al
+adox r10, [ rsp - 0x20 ]
+adox rdi, [ rsp - 0x28 ]
+shrd rbx, r9, 52
+mov r11, rbp
+shrd r11, r15, 52
+xor r9, r9
+adox rbx, r10
+adox rdi, r9
+adcx r14, rbx
+adcx rdi, rcx
+mov r15, r14
+shrd r15, rdi, 52
+mov rdx, [ rsi + 0x8 ]
+mulx r10, rcx, [ rax + 0x8 ]
+mov rdx, 0xfffffffffffff 
+and r14, rdx
+mov rbx, 0x1000003d10 
+mov rdx, rbx
+mulx rdi, rbx, r11
+mov r11, rcx
+adox r11, [ rsp - 0x40 ]
+adox r10, [ rsp - 0x48 ]
+mov rcx, 0x34 
+bzhi r9, rbp, rcx
+adox r11, [ rsp - 0x30 ]
+adox r10, [ rsp - 0x38 ]
+xor rbp, rbp
+adox r15, r11
+adox r10, rbp
+mulx rbp, r11, r9
+adcx r11, r15
+adcx r10, rbp
+bzhi r9, r11, rcx
+mov r15, [ rsp - 0x50 ]
+mov [ r15 + 0x10 ], r9
+shrd r11, r10, 52
+lea r12, [ r12 + r11 ]
+xor rbp, rbp
+adox rbx, r12
+adox rdi, rbp
+bzhi r10, rbx, rcx
+mov [ r15 + 0x8 ], r14
+shrd rbx, rdi, 52
+lea r13, [ r13 + rbx ]
+mov [ r15 + 0x0 ], r8
+mov [ r15 + 0x20 ], r13
+mov [ r15 + 0x18 ], r10
+mov rbx, [ rsp - 0x80 ]
+mov rbp, [ rsp - 0x78 ]
+mov r12, [ rsp - 0x70 ]
+mov r13, [ rsp - 0x68 ]
+mov r14, [ rsp - 0x60 ]
+mov r15, [ rsp - 0x58 ]
+ret
+; cpu Intel(R) Core(TM) i7-10710U CPU @ 1.10GHz
+; ratio 1.0725
+; seed 1206382180236178 
+; CC / CFLAGS clang / -march=native -mtune=native -O3 
+; time needed: 1957870 ms on 180000 evaluations.
+; Time spent for assembling and measuring (initial batch_size=339, initial num_batches=31): 164549 ms
+; number of used evaluations: 180000
+; Ratio (time for assembling + measure)/(total runtime for 180000 evals): 0.08404490594370413
+; number reverted permutation / tried permutation: 70311 / 90024 =78.103%
+; number reverted decision / tried decision: 51961 / 89975 =57.750%
+; validated in 0.713s
