fiat-amd64/fiat_secp256k1_dettman_square/seed0000000063664254_ratio09742.asm
@@ -1,0 +1,175 @@
+SECTION .text
+	GLOBAL fiat_secp256k1_dettman_square
+fiat_secp256k1_dettman_square:
+mov rax, [ rsi + 0x8 ]
+mov r10, rax
+shl r10, 0x1
+mov rdx, [ rsi + 0x20 ]
+mulx r11, rax, rdx
+mov rdx, [ rsi + 0x10 ]
+mulx r8, rcx, rdx
+mov rdx, [ rsi + 0x0 ]
+lea r9, [rdx + rdx]
+mov rdx, 0xfffffffffffff 
+mov [ rsp - 0x80 ], rbx
+mov rbx, rax
+and rbx, rdx
+mov rdx, r9
+mov [ rsp - 0x78 ], rbp
+mulx rbp, r9, [ rsi + 0x20 ]
+mov [ rsp - 0x70 ], r12
+mov r12, 0x1000003d10 
+xchg rdx, rbx
+mov [ rsp - 0x68 ], r13
+mov [ rsp - 0x60 ], r14
+mulx r14, r13, r12
+shrd rax, r11, 52
+mov rdx, [ rsi + 0x18 ]
+mov [ rsp - 0x58 ], r15
+mulx r15, r11, rbx
+mov rdx, [ rsi + 0x10 ]
+mov [ rsp - 0x50 ], rdi
+mulx rdi, r12, r10
+xor rdx, rdx
+adox r12, r11
+adox r15, rdi
+adcx r13, r12
+adcx r15, r14
+mov rdx, [ rsi + 0x10 ]
+mulx r11, r14, rbx
+mov rdx, [ rsi + 0x8 ]
+mulx r12, rdi, rdx
+add rdi, r14
+adcx r11, r12
+mov rdx, r10
+mulx r14, r10, [ rsi + 0x18 ]
+xor r12, r12
+adox rcx, r10
+adox r14, r8
+mov r8, 0x1 
+shlx r10, [ rsi + 0x10 ], r8
+mov r12, rdx
+mov rdx, [ rsi + 0x18 ]
+mov [ rsp - 0x48 ], r11
+mulx r11, r8, r10
+adcx rcx, r9
+adcx rbp, r14
+mov rdx, 0xfffffffffffff 
+mov r9, r13
+and r9, rdx
+mov r14, 0x1000003d10 
+mov rdx, rax
+mov [ rsp - 0x40 ], r9
+mulx r9, rax, r14
+shrd r13, r15, 52
+add r13, rcx
+adc rbp, 0x0
+test al, al
+adox rax, r13
+adox rbp, r9
+mov rdx, rax
+shrd rdx, rbp, 52
+xchg rdx, r12
+mulx rcx, r15, [ rsi + 0x20 ]
+xor rdx, rdx
+adox r8, r15
+adox rcx, r11
+adcx r12, r8
+adc rcx, 0x0
+mov r11, 0xfffffffffffff 
+mov r9, r12
+and r9, r11
+shrd r12, rcx, 52
+and rax, r11
+mov r13, rax
+shr r13, 48
+shl r9, 4
+mov rdx, [ rsi + 0x18 ]
+mulx r15, rbp, rdx
+mov rdx, 0xffffffffffff 
+and rax, rdx
+mov rdx, r10
+mulx r8, r10, [ rsi + 0x20 ]
+adox rbp, r10
+adox r8, r15
+mov rdx, [ rsi + 0x18 ]
+mov rcx, rdx
+shl rcx, 0x1
+lea r9, [ r9 + r13 ]
+mov rdx, [ rsi + 0x0 ]
+mulx r15, r13, rdx
+mov rdx, 0x1000003d1 
+mulx r14, r10, r9
+xor r9, r9
+adox r10, r13
+adox r15, r14
+mov r13, r10
+shrd r13, r15, 52
+test al, al
+adox r12, rbp
+adox r8, r9
+mov rbp, r12
+shrd rbp, r8, 52
+and r10, r11
+mov rdx, [ rsi + 0x8 ]
+mulx r15, r14, rbx
+adox r13, r14
+adox r15, r9
+and r12, r11
+mov rdx, [ rsi + 0x20 ]
+mulx r8, rbx, rcx
+adox rbp, rbx
+adox r8, r9
+mov rdx, rbp
+shrd rdx, r8, 52
+mov rcx, 0x1000003d10 
+mulx rbx, r14, rcx
+mov rdx, rcx
+mulx r8, rcx, r12
+test al, al
+adox rcx, r13
+adox r15, r8
+mov r13, rcx
+shrd r13, r15, 52
+and rbp, r11
+mulx r8, r12, rbp
+adox r13, rdi
+mov r15, [ rsp - 0x48 ]
+adox r15, r9
+adcx r12, r13
+adcx r15, r8
+mov rdi, [ rsp - 0x50 ]
+mov [ rdi + 0x0 ], r10
+mov r10, r12
+shrd r10, r15, 52
+add r10, [ rsp - 0x40 ]
+add r14, r10
+adc rbx, 0x0
+and r12, r11
+mov rbp, r14
+shrd rbp, rbx, 52
+and r14, r11
+mov [ rdi + 0x18 ], r14
+and rcx, r11
+lea rax, [ rax + rbp ]
+mov [ rdi + 0x8 ], rcx
+mov [ rdi + 0x20 ], rax
+mov [ rdi + 0x10 ], r12
+mov rbx, [ rsp - 0x80 ]
+mov rbp, [ rsp - 0x78 ]
+mov r12, [ rsp - 0x70 ]
+mov r13, [ rsp - 0x68 ]
+mov r14, [ rsp - 0x60 ]
+mov r15, [ rsp - 0x58 ]
+ret
+; cpu AMD Ryzen 7 5800X 8-Core Processor
+; ratio 0.9742
+; seed 3076211693309636 
+; CC / CFLAGS clang / -march=native -mtune=native -O3 
+; time needed: 918299 ms on 180000 evaluations.
+; Time spent for assembling and measuring (initial batch_size=252, initial num_batches=31): 81168 ms
+; number of used evaluations: 180000
+; Ratio (time for assembling + measure)/(total runtime for 180000 evals): 0.0883895114771986
+; number reverted permutation / tried permutation: 75974 / 89835 =84.571%
+; number reverted decision / tried decision: 54417 / 90164 =60.353%
+; validated in 0.253s
