fiat-amd64/fiat_secp256k1_dettman_square/seed0000000225267441_ratio09530.asm
@@ -1,0 +1,174 @@
+SECTION .text
+	GLOBAL fiat_secp256k1_dettman_square
+fiat_secp256k1_dettman_square:
+mov rdx, [ rsi + 0x20 ]
+mulx r10, rax, rdx
+mov r11, [ rsi + 0x0 ]
+lea rdx, [r11 + r11]
+mov r11, rdx
+mov rdx, [ rsi + 0x18 ]
+mulx r8, rcx, rdx
+mov rdx, [ rsi + 0x18 ]
+mov [ rsp - 0x80 ], rbx
+mulx rbx, r9, r11
+mov rdx, [ rsi + 0x8 ]
+mov [ rsp - 0x78 ], rbp
+mov rbp, rdx
+shl rbp, 0x1
+mov rdx, [ rsi + 0x10 ]
+mov [ rsp - 0x70 ], r12
+mov [ rsp - 0x68 ], r13
+mulx r13, r12, rbp
+test al, al
+adox r12, r9
+adox rbx, r13
+mov rdx, rax
+shrd rdx, r10, 52
+mov r10, 0xfffffffffffff 
+and rax, r10
+xchg rdx, rbp
+mulx r13, r9, [ rsi + 0x18 ]
+mov [ rsp - 0x60 ], r14
+mov r14, rdx
+mov rdx, [ rsi + 0x10 ]
+mov [ rsp - 0x58 ], r15
+mulx r10, r15, rdx
+adox r15, r9
+adox r13, r10
+mov rdx, [ rsi + 0x20 ]
+mulx r10, r9, r11
+adcx r15, r9
+adcx r10, r13
+mov rdx, 0x1000003d10 
+mulx r9, r13, rax
+test al, al
+adox r13, r12
+adox rbx, r9
+mov r12, r13
+shrd r12, rbx, 52
+add r12, r15
+adc r10, 0x0
+mulx r15, rax, rbp
+xor rbp, rbp
+adox rax, r12
+adox r10, r15
+mov r9, 0x1 
+shlx rbx, [ rsi + 0x10 ], r9
+mov r12, rax
+shrd r12, r10, 52
+mov rdx, [ rsi + 0x18 ]
+mulx r10, r15, rbx
+mov rdx, [ rsi + 0x20 ]
+mulx r9, rbp, r14
+xor rdx, rdx
+adox r15, rbp
+adox r9, r10
+mov r14, 0x34 
+bzhi r10, r13, r14
+adox r12, r15
+adox r9, rdx
+bzhi r13, r12, r14
+shrd r12, r9, 52
+bzhi rbp, rax, r14
+shl r13, 4
+mov rax, 0xffffffffffff 
+mov r15, rbp
+and r15, rax
+mov rdx, [ rsi + 0x20 ]
+mulx r14, r9, rbx
+adox rcx, r9
+adox r14, r8
+shr rbp, 48
+mov rdx, [ rsi + 0x18 ]
+mov r8, rdx
+shl r8, 0x1
+lea r13, [ r13 + rbp ]
+xor rdx, rdx
+adox r12, rcx
+adox r14, rdx
+mov rdx, [ rsi + 0x0 ]
+mulx r9, rbx, rdx
+mov rdx, r8
+mulx rcx, r8, [ rsi + 0x20 ]
+mov rbp, r12
+shrd rbp, r14, 52
+test al, al
+adox rbp, r8
+mov rdx, 0x0 
+adox rcx, rdx
+mov r14, 0x1000003d1 
+mov rdx, r13
+mulx r8, r13, r14
+mov rdx, [ rsi + 0x8 ]
+mulx rax, r14, rdx
+adcx r13, rbx
+adcx r9, r8
+mov rdx, rbp
+shrd rdx, rcx, 52
+mov rbx, 0xfffffffffffff 
+mov rcx, r13
+and rcx, rbx
+mov r8, rdx
+mov rdx, [ rsi + 0x10 ]
+mov [ rsp - 0x50 ], rdi
+mulx rdi, rbx, r11
+adox r14, rbx
+adox rdi, rax
+mov rdx, [ rsi + 0x8 ]
+mulx rbx, rax, r11
+mov rdx, 0xfffffffffffff 
+and r12, rdx
+mov r11, [ rsp - 0x50 ]
+mov [ r11 + 0x0 ], rcx
+mov rcx, 0x1000003d10 
+mov rdx, rcx
+mulx r11, rcx, r12
+shrd r13, r9, 52
+xor r9, r9
+adox r13, rax
+adox rbx, r9
+adcx rcx, r13
+adcx rbx, r11
+mov rax, 0x34 
+bzhi r12, rbp, rax
+bzhi rbp, rcx, rax
+shrd rcx, rbx, 52
+mulx r13, r11, r12
+add rcx, r14
+adc rdi, 0x0
+add r11, rcx
+adcx rdi, r13
+mov r14, r11
+shrd r14, rdi, 52
+bzhi rbx, r11, rax
+mov r12, [ rsp - 0x50 ]
+mov [ r12 + 0x10 ], rbx
+lea r10, [ r10 + r14 ]
+mulx rcx, r13, r8
+adox r13, r10
+adox rcx, r9
+mov r8, r13
+shrd r8, rcx, 52
+lea r15, [ r15 + r8 ]
+mov [ r12 + 0x20 ], r15
+bzhi r11, r13, rax
+mov [ r12 + 0x8 ], rbp
+mov [ r12 + 0x18 ], r11
+mov rbx, [ rsp - 0x80 ]
+mov rbp, [ rsp - 0x78 ]
+mov r12, [ rsp - 0x70 ]
+mov r13, [ rsp - 0x68 ]
+mov r14, [ rsp - 0x60 ]
+mov r15, [ rsp - 0x58 ]
+ret
+; cpu AMD Ryzen 9 7950X 16-Core Processor
+; ratio 0.9530
+; seed 2351914705828844 
+; CC / CFLAGS clang / -march=native -mtune=native -O3 
+; time needed: 696387 ms on 180000 evaluations.
+; Time spent for assembling and measuring (initial batch_size=243, initial num_batches=31): 67405 ms
+; number of used evaluations: 180000
+; Ratio (time for assembling + measure)/(total runtime for 180000 evals): 0.09679244443104193
+; number reverted permutation / tried permutation: 74949 / 89949 =83.324%
+; number reverted decision / tried decision: 60622 / 90050 =67.320%
+; validated in 0.199s
