fiat-amd64/fiat_secp256k1_dettman_square/seed0000000583341977_ratio11387.asm
@@ -1,0 +1,175 @@
+SECTION .text
+	GLOBAL fiat_secp256k1_dettman_square
+fiat_secp256k1_dettman_square:
+mov rax, 0x1 
+shlx r10, [ rsi + 0x8 ], rax
+mov rdx, [ rsi + 0x20 ]
+mulx rcx, r11, rdx
+mov rdx, r11
+shrd rdx, rcx, 52
+mov r8, 0x1000003d10 
+mulx rcx, r9, r8
+shlx rdx, [ rsi + 0x10 ], rax
+mov rax, rdx
+mov rdx, [ rsi + 0x18 ]
+mov [ rsp - 0x80 ], rbx
+mov [ rsp - 0x78 ], rbp
+mulx rbp, rbx, rdx
+mov rdx, 0x34 
+mov [ rsp - 0x70 ], r12
+bzhi r12, r11, rdx
+mov r11, [ rsi + 0x0 ]
+mov [ rsp - 0x68 ], r13
+lea r13, [r11 + r11]
+mov rdx, r13
+mulx r13, r11, [ rsi + 0x18 ]
+mov [ rsp - 0x60 ], r14
+mov r14, rdx
+mov rdx, [ rsi + 0x10 ]
+mov [ rsp - 0x58 ], r15
+mulx r8, r15, r10
+adox r15, r11
+adox r13, r8
+mov rdx, [ rsi + 0x18 ]
+mulx r8, r11, r10
+mov rdx, [ rsi + 0x10 ]
+mov [ rsp - 0x50 ], rdi
+mov [ rsp - 0x48 ], rbp
+mulx rbp, rdi, rdx
+xor rdx, rdx
+adox rdi, r11
+adox r8, rbp
+mov r11, 0x1000003d10 
+mov rdx, r11
+mulx rbp, r11, r12
+adcx r11, r15
+adcx r13, rbp
+mov rdx, r14
+mulx r12, r14, [ rsi + 0x20 ]
+mov r15, rdx
+mov rdx, [ rsi + 0x18 ]
+mov [ rsp - 0x40 ], rbx
+mulx rbx, rbp, rax
+xor rdx, rdx
+adox rdi, r14
+adox r12, r8
+mov rdx, [ rsi + 0x20 ]
+mulx r14, r8, r10
+adcx rbp, r8
+adcx r14, rbx
+mov rdx, r11
+shrd rdx, r13, 52
+add rdx, rdi
+adc r12, 0x0
+xor r10, r10
+adox r9, rdx
+adox r12, rcx
+mov rcx, r9
+shrd rcx, r12, 52
+mov rdx, [ rsi + 0x20 ]
+mulx rbx, r13, rax
+add rcx, rbp
+adc r14, 0x0
+mov rdx, rcx
+shrd rdx, r14, 52
+mov rax, r13
+xor rdi, rdi
+adox rax, [ rsp - 0x40 ]
+adox rbx, [ rsp - 0x48 ]
+adcx rdx, rax
+adc rbx, 0x0
+mov r10, rdx
+shrd r10, rbx, 52
+mov r8, 0x34 
+bzhi rbp, r9, r8
+mov r9, rbp
+shr r9, 48
+mov r12, [ rsi + 0x18 ]
+lea r13, [r12 + r12]
+mov r12, 0x30 
+bzhi r14, rbp, r12
+mov rax, rdx
+mov rdx, [ rsi + 0x20 ]
+mulx rbp, rbx, r13
+adox r10, rbx
+adox rbp, rdi
+bzhi rdx, rcx, r8
+shl rdx, 4
+lea rdx, [ rdx + r9 ]
+mov rcx, r10
+shrd rcx, rbp, 52
+bzhi r9, rax, r8
+mov rax, 0x1000003d1 
+mulx rbx, r13, rax
+mov rdx, [ rsi + 0x0 ]
+mulx rdi, rbp, rdx
+mov rdx, 0x1000003d10 
+mulx r8, r12, r9
+adox r13, rbp
+adox rdi, rbx
+mov r9, r13
+shrd r9, rdi, 52
+mov rdx, [ rsi + 0x8 ]
+mulx rbp, rbx, r15
+add r9, rbx
+adc rbp, 0x0
+xor rdx, rdx
+adox r12, r9
+adox rbp, r8
+mov rdx, [ rsi + 0x8 ]
+mulx rdi, r8, rdx
+mov rdx, [ rsi + 0x10 ]
+mulx r9, rbx, r15
+adcx r8, rbx
+adcx r9, rdi
+mov rdx, 0xfffffffffffff 
+and r13, rdx
+mov r15, [ rsp - 0x50 ]
+mov [ r15 + 0x0 ], r13
+mov rdi, r12
+shrd rdi, rbp, 52
+and r11, rdx
+adox rdi, r8
+mov rbp, 0x0 
+adox r9, rbp
+and r10, rdx
+mov rbx, 0x1000003d10 
+mov rdx, r10
+mulx r8, r10, rbx
+adox r10, rdi
+adox r9, r8
+mov r13, 0x34 
+bzhi rdi, r10, r13
+shrd r10, r9, 52
+lea r11, [ r11 + r10 ]
+mov rdx, rcx
+mulx r8, rcx, rbx
+add rcx, r11
+adc r8, 0x0
+mov rdx, rcx
+shrd rdx, r8, 52
+lea r14, [ r14 + rdx ]
+mov [ r15 + 0x20 ], r14
+bzhi r9, rcx, r13
+mov [ r15 + 0x18 ], r9
+mov [ r15 + 0x10 ], rdi
+bzhi rdi, r12, r13
+mov [ r15 + 0x8 ], rdi
+mov rbx, [ rsp - 0x80 ]
+mov rbp, [ rsp - 0x78 ]
+mov r12, [ rsp - 0x70 ]
+mov r13, [ rsp - 0x68 ]
+mov r14, [ rsp - 0x60 ]
+mov r15, [ rsp - 0x58 ]
+ret
+; cpu 11th Gen Intel(R) Core(TM) i7-11700KF @ 3.60GHz
+; ratio 1.1387
+; seed 3566223694906793 
+; CC / CFLAGS clang / -march=native -mtune=native -O3 
+; time needed: 936820 ms on 180000 evaluations.
+; Time spent for assembling and measuring (initial batch_size=284, initial num_batches=31): 77550 ms
+; number of used evaluations: 180000
+; Ratio (time for assembling + measure)/(total runtime for 180000 evals): 0.08278004312461305
+; number reverted permutation / tried permutation: 74935 / 89702 =83.538%
+; number reverted decision / tried decision: 64943 / 90297 =71.922%
+; validated in 0.302s
