fiat-amd64/fiat_secp256k1_dettman_square/seed2625400661231680_ratio11844.asm
@@ -1,0 +1,174 @@
+SECTION .text
+	GLOBAL fiat_secp256k1_dettman_square
+fiat_secp256k1_dettman_square:
+mov rax, [ rsi + 0x8 ]
+lea r10, [rax + rax]
+mov rax, [ rsi + 0x0 ]
+mov r11, rax
+shl r11, 0x1
+mov rdx, [ rsi + 0x20 ]
+mulx rcx, rax, rdx
+mov rdx, r11
+mulx r8, r11, [ rsi + 0x18 ]
+mov r9, rdx
+mov rdx, [ rsi + 0x18 ]
+mov [ rsp - 0x80 ], rbx
+mov [ rsp - 0x78 ], rbp
+mulx rbp, rbx, r10
+mov rdx, r10
+mov [ rsp - 0x70 ], r12
+mulx r12, r10, [ rsi + 0x10 ]
+mov [ rsp - 0x68 ], r13
+xor r13, r13
+adox r10, r11
+adox r8, r12
+mov r11, [ rsi + 0x10 ]
+lea r12, [r11 + r11]
+mov r11, 0xfffffffffffff 
+mov r13, rax
+and r13, r11
+mov [ rsp - 0x60 ], r14
+mov [ rsp - 0x58 ], r15
+mulx r15, r14, [ rsi + 0x20 ]
+mov rdx, 0x1000003d10 
+mov [ rsp - 0x50 ], rdi
+mulx rdi, r11, r13
+mov rdx, [ rsi + 0x10 ]
+mov [ rsp - 0x48 ], r15
+mulx r15, r13, rdx
+adox r11, r10
+adox r8, rdi
+shrd rax, rcx, 52
+mov rdx, [ rsi + 0x20 ]
+mulx r10, rcx, r9
+mov rdx, 0x1000003d10 
+mov [ rsp - 0x40 ], r14
+mulx r14, rdi, rax
+add r13, rbx
+adcx rbp, r15
+mov rbx, r11
+shrd rbx, r8, 52
+xor r15, r15
+adox r13, rcx
+adox r10, rbp
+mov rdx, [ rsi + 0x8 ]
+mulx rax, r8, rdx
+mov rdx, [ rsi + 0x18 ]
+mov rcx, rdx
+shl rcx, 0x1
+mov rdx, r12
+mulx rbp, r12, [ rsi + 0x18 ]
+mov r15, rdx
+mov rdx, [ rsi + 0x20 ]
+mov [ rsp - 0x38 ], rax
+mov [ rsp - 0x30 ], r8
+mulx r8, rax, rcx
+xor rdx, rdx
+adox r12, [ rsp - 0x40 ]
+adox rbp, [ rsp - 0x48 ]
+adcx rbx, r13
+adc r10, 0x0
+mov rdx, [ rsi + 0x18 ]
+mulx rcx, r13, rdx
+add rdi, rbx
+adcx r10, r14
+mov rdx, [ rsi + 0x20 ]
+mulx rbx, r14, r15
+xor rdx, rdx
+adox r13, r14
+adox rbx, rcx
+mov r15, 0xfffffffffffff 
+mov rcx, rdi
+and rcx, r15
+shrd rdi, r10, 52
+add rdi, r12
+adc rbp, 0x0
+mov r12, rdi
+shrd r12, rbp, 52
+and rdi, r15
+adox r12, r13
+adox rbx, rdx
+mov r10, 0xffffffffffff 
+mov r14, rcx
+and r14, r10
+shl rdi, 4
+shr rcx, 48
+mov r13, r12
+shrd r13, rbx, 52
+lea rdi, [ rdi + rcx ]
+and r12, r15
+adox r13, rax
+adox r8, rdx
+mov rax, 0x1000003d10 
+mov rdx, rax
+mulx rbp, rax, r12
+mov rbx, r13
+and rbx, r15
+shrd r13, r8, 52
+mulx r12, rcx, rbx
+mulx rbx, r8, r13
+mov rdx, [ rsi + 0x0 ]
+mulx r10, r13, rdx
+mov rdx, 0x1000003d1 
+mov [ rsp - 0x28 ], r14
+mulx r14, r15, rdi
+xor rdi, rdi
+adox r15, r13
+adox r10, r14
+mov r13, r15
+shrd r13, r10, 52
+mov rdx, r9
+mulx r14, r9, [ rsi + 0x8 ]
+mov r10, 0xfffffffffffff 
+and r15, r10
+adox r13, r9
+adox r14, rdi
+adcx rax, r13
+adcx r14, rbp
+mov rbp, rax
+shrd rbp, r14, 52
+and rax, r10
+mov r9, [ rsp - 0x50 ]
+mov [ r9 + 0x0 ], r15
+mulx r13, r15, [ rsi + 0x10 ]
+mov [ r9 + 0x8 ], rax
+and r11, r10
+mov rdx, r15
+adox rdx, [ rsp - 0x30 ]
+adox r13, [ rsp - 0x38 ]
+adcx rbp, rdx
+adc r13, 0x0
+xor r14, r14
+adox rcx, rbp
+adox r13, r12
+mov rdi, rcx
+shrd rdi, r13, 52
+and rcx, r10
+lea r11, [ r11 + rdi ]
+adox r8, r11
+adox rbx, r14
+mov r12, r8
+shrd r12, rbx, 52
+add r12, [ rsp - 0x28 ]
+and r8, r10
+mov [ r9 + 0x18 ], r8
+mov [ r9 + 0x20 ], r12
+mov [ r9 + 0x10 ], rcx
+mov rbx, [ rsp - 0x80 ]
+mov rbp, [ rsp - 0x78 ]
+mov r12, [ rsp - 0x70 ]
+mov r13, [ rsp - 0x68 ]
+mov r14, [ rsp - 0x60 ]
+mov r15, [ rsp - 0x58 ]
+ret
+; cpu 12th Gen Intel(R) Core(TM) i9-12900KF
+; ratio 1.1844
+; seed 2625400661231680 
+; CC / CFLAGS clang / -march=native -mtune=native -O3 
+; time needed: 4420 ms on 1000 evaluations.
+; Time spent for assembling and measuring (initial batch_size=367, initial num_batches=31): 446 ms
+; number of used evaluations: 1000
+; Ratio (time for assembling + measure)/(total runtime for 1000 evals): 0.10090497737556561
+; number reverted permutation / tried permutation: 369 / 483 =76.398%
+; number reverted decision / tried decision: 351 / 516 =68.023%
+; validated in 0.197s
