fiat-amd64/fiat_secp256k1_dettman_square/seed2716647052398798_ratio11133.asm
@@ -1,0 +1,179 @@
+SECTION .text
+	GLOBAL fiat_secp256k1_dettman_square
+fiat_secp256k1_dettman_square:
+mov rdx, [ rsi + 0x10 ]
+mulx r10, rax, rdx
+mov r11, [ rsi + 0x18 ]
+lea rdx, [r11 + r11]
+mov r11, 0x1 
+shlx rcx, [ rsi + 0x10 ], r11
+mov r8, rdx
+mov rdx, [ rsi + 0x20 ]
+mulx r11, r9, rdx
+mov rdx, rcx
+mov [ rsp - 0x80 ], rbx
+mulx rbx, rcx, [ rsi + 0x18 ]
+mov [ rsp - 0x78 ], rbp
+mov rbp, 0x34 
+mov [ rsp - 0x70 ], r12
+bzhi r12, r9, rbp
+mov [ rsp - 0x68 ], r13
+mov r13, [ rsi + 0x8 ]
+mov [ rsp - 0x60 ], r14
+mov r14, r13
+shl r14, 0x1
+shrd r9, r11, 52
+mov r13, [ rsi + 0x0 ]
+mov r11, r13
+shl r11, 0x1
+mov r13, rdx
+mov rdx, [ rsi + 0x18 ]
+mov [ rsp - 0x58 ], r15
+mulx rbp, r15, r14
+mov rdx, r11
+mov [ rsp - 0x50 ], rdi
+mulx rdi, r11, [ rsi + 0x18 ]
+mov [ rsp - 0x48 ], r9
+mov [ rsp - 0x40 ], r8
+mulx r8, r9, [ rsi + 0x10 ]
+mov [ rsp - 0x38 ], r8
+mov r8, rdx
+mov rdx, [ rsi + 0x10 ]
+mov [ rsp - 0x30 ], r9
+mov [ rsp - 0x28 ], rbx
+mulx rbx, r9, r14
+xor rdx, rdx
+adox r9, r11
+adox rdi, rbx
+adcx rax, r15
+adcx rbp, r10
+mov rdx, r8
+mulx r10, r8, [ rsi + 0x20 ]
+mov r15, rdx
+mov rdx, [ rsi + 0x20 ]
+mulx rbx, r11, r13
+mov rdx, [ rsi + 0x18 ]
+mov [ rsp - 0x20 ], rbp
+mulx rbp, r13, rdx
+xor rdx, rdx
+adox r13, r11
+adox rbx, rbp
+mov r11, 0x1000003d10 
+mov rdx, r12
+mulx rbp, r12, r11
+adcx r12, r9
+adcx rdi, rbp
+mov rdx, [ rsi + 0x20 ]
+mulx rbp, r9, r14
+xor rdx, rdx
+adox rcx, r9
+adox rbp, [ rsp - 0x28 ]
+mov r14, r12
+shrd r14, rdi, 52
+add rax, r8
+adcx r10, [ rsp - 0x20 ]
+mov rdx, [ rsp - 0x40 ]
+mulx rdi, r8, [ rsi + 0x20 ]
+xor rdx, rdx
+adox r14, rax
+adox r10, rdx
+mov rdx, [ rsp - 0x48 ]
+mulx rax, r9, r11
+adcx r9, r14
+adcx r10, rax
+mov rdx, 0xfffffffffffff 
+mov r14, r9
+and r14, rdx
+and r12, rdx
+shrd r9, r10, 52
+xor rax, rax
+adox r9, rcx
+adox rbp, rax
+mov rcx, r9
+shrd rcx, rbp, 52
+mov r10, r14
+shr r10, 48
+mov rbp, 0xffffffffffff 
+and r14, rbp
+adox rcx, r13
+adox rbx, rax
+mov rdx, [ rsi + 0x0 ]
+mulx rax, r13, rdx
+mov rdx, 0xfffffffffffff 
+mov rbp, rcx
+and rbp, rdx
+and r9, rdx
+shl r9, 4
+lea r9, [ r9 + r10 ]
+shrd rcx, rbx, 52
+mov r10, 0x1000003d1 
+mov rdx, r10
+mulx rbx, r10, r9
+xor r9, r9
+adox r10, r13
+adox rax, rbx
+adcx rcx, r8
+adc rdi, 0x0
+mov r8, 0x34 
+bzhi r13, r10, r8
+mov rbx, [ rsp - 0x50 ]
+mov [ rbx + 0x0 ], r13
+mov rdx, [ rsi + 0x8 ]
+mulx r9, r13, rdx
+mov rdx, [ rsi + 0x8 ]
+mulx r11, r8, r15
+adox r13, [ rsp - 0x30 ]
+adox r9, [ rsp - 0x38 ]
+mov rdx, 0x1000003d10 
+mulx rbx, r15, rbp
+shrd r10, rax, 52
+mov rbp, rcx
+shrd rbp, rdi, 52
+xor rax, rax
+adox r10, r8
+adox r11, rax
+adcx r15, r10
+adcx r11, rbx
+mov rdi, r15
+shrd rdi, r11, 52
+test al, al
+adox rdi, r13
+adox r9, rax
+mulx r13, r8, rbp
+mov rbx, 0x34 
+bzhi rbp, rcx, rbx
+mulx r10, rcx, rbp
+adox rcx, rdi
+adox r9, r10
+bzhi r11, rcx, rbx
+shrd rcx, r9, 52
+mov rdi, [ rsp - 0x50 ]
+mov [ rdi + 0x10 ], r11
+lea r12, [ r12 + rcx ]
+add r8, r12
+adc r13, 0x0
+bzhi rbp, r8, rbx
+mov [ rdi + 0x18 ], rbp
+shrd r8, r13, 52
+lea r14, [ r14 + r8 ]
+bzhi r10, r15, rbx
+mov [ rdi + 0x8 ], r10
+mov [ rdi + 0x20 ], r14
+mov rbx, [ rsp - 0x80 ]
+mov rbp, [ rsp - 0x78 ]
+mov r12, [ rsp - 0x70 ]
+mov r13, [ rsp - 0x68 ]
+mov r14, [ rsp - 0x60 ]
+mov r15, [ rsp - 0x58 ]
+ret
+; cpu 11th Gen Intel(R) Core(TM) i7-11700KF @ 3.60GHz
+; ratio 1.1133
+; seed 2716647052398798 
+; CC / CFLAGS clang / -march=native -mtune=native -O3 
+; time needed: 5474 ms on 1000 evaluations.
+; Time spent for assembling and measuring (initial batch_size=280, initial num_batches=31): 458 ms
+; number of used evaluations: 1000
+; Ratio (time for assembling + measure)/(total runtime for 1000 evals): 0.08366824990865912
+; number reverted permutation / tried permutation: 427 / 527 =81.025%
+; number reverted decision / tried decision: 320 / 472 =67.797%
+; validated in 0.31s
