fiat-amd64/fiat_secp256k1_dettman_square/seed3093611607776169_ratio09742.asm
@@ -1,0 +1,176 @@
+SECTION .text
+	GLOBAL fiat_secp256k1_dettman_square
+fiat_secp256k1_dettman_square:
+mov rdx, [ rsi + 0x20 ]
+mulx r10, rax, rdx
+mov r11, [ rsi + 0x10 ]
+lea rdx, [r11 + r11]
+mulx rcx, r11, [ rsi + 0x20 ]
+mov r8, rax
+shrd r8, r10, 52
+mulx r10, r9, [ rsi + 0x18 ]
+mov rdx, [ rsi + 0x0 ]
+mov [ rsp - 0x80 ], rbx
+lea rbx, [rdx + rdx]
+mov rdx, [ rsi + 0x20 ]
+mov [ rsp - 0x78 ], rbp
+mov [ rsp - 0x70 ], r12
+mulx r12, rbp, rbx
+mov rdx, rbx
+mov [ rsp - 0x68 ], r13
+mulx r13, rbx, [ rsi + 0x18 ]
+mov [ rsp - 0x60 ], r14
+mov r14, [ rsi + 0x18 ]
+mov [ rsp - 0x58 ], r15
+mov r15, r14
+shl r15, 0x1
+imul r14, [ rsi + 0x8 ], 0x2
+xchg rdx, r14
+mov [ rsp - 0x50 ], rdi
+mov [ rsp - 0x48 ], r15
+mulx r15, rdi, [ rsi + 0x10 ]
+mov [ rsp - 0x40 ], r8
+xor r8, r8
+adox rdi, rbx
+adox r13, r15
+mov rbx, 0x34 
+bzhi r15, rax, rbx
+mov rax, 0x1000003d10 
+xchg rdx, r15
+mulx rbx, r8, rax
+mov rdx, r14
+mulx rax, r14, [ rsi + 0x10 ]
+mov [ rsp - 0x38 ], rax
+mov rax, rdx
+mov rdx, [ rsi + 0x18 ]
+mov [ rsp - 0x30 ], r14
+mov [ rsp - 0x28 ], r12
+mulx r12, r14, rdx
+adox r14, r11
+adox rcx, r12
+mov rdx, [ rsi + 0x8 ]
+mulx r12, r11, rdx
+test al, al
+adox r8, rdi
+adox r13, rbx
+mov rdx, [ rsi + 0x20 ]
+mulx rbx, rdi, r15
+mov rdx, 0xfffffffffffff 
+mov [ rsp - 0x20 ], r12
+mov r12, r8
+and r12, rdx
+adox r9, rdi
+adox rbx, r10
+mov rdx, [ rsi + 0x10 ]
+mulx rdi, r10, rdx
+mov rdx, [ rsi + 0x18 ]
+mov [ rsp - 0x18 ], r12
+mov [ rsp - 0x10 ], r11
+mulx r11, r12, r15
+adcx r10, r12
+adcx r11, rdi
+xor rdx, rdx
+adox r10, rbp
+adox r11, [ rsp - 0x28 ]
+shrd r8, r13, 52
+mov rbp, 0x1000003d10 
+mov rdx, [ rsp - 0x40 ]
+mulx r13, r15, rbp
+xor rdx, rdx
+adox r8, r10
+adox r11, rdx
+adcx r15, r8
+adcx r11, r13
+mov rdi, r15
+shrd rdi, r11, 52
+mov r12, 0xfffffffffffff 
+and r15, r12
+adox rdi, r9
+adox rbx, rdx
+mov r9, rdi
+shrd r9, rbx, 52
+and rdi, r12
+shl rdi, 4
+mov r10, r15
+shr r10, 48
+mov rdx, [ rsi + 0x0 ]
+mulx r8, r13, rdx
+lea rdi, [ rdi + r10 ]
+mov rdx, 0x1000003d1 
+mulx rbx, r11, rdi
+mov r10, 0xffffffffffff 
+and r15, r10
+mov rdx, [ rsi + 0x8 ]
+mulx r10, rdi, rax
+adox r9, r14
+mov rdx, 0x0 
+adox rcx, rdx
+adcx r11, r13
+adcx r8, rbx
+mov rax, r11
+and rax, r12
+mov r14, r9
+shrd r14, rcx, 52
+mov r13, [ rsp - 0x50 ]
+mov [ r13 + 0x0 ], rax
+and r9, r12
+mov rdx, [ rsi + 0x20 ]
+mulx rcx, rbx, [ rsp - 0x48 ]
+mov rdx, rbp
+mulx rax, rbp, r9
+shrd r11, r8, 52
+add r14, rbx
+adc rcx, 0x0
+mov r8, r14
+and r8, r12
+mov r9, [ rsp - 0x10 ]
+adox r9, [ rsp - 0x30 ]
+mov rbx, [ rsp - 0x20 ]
+adox rbx, [ rsp - 0x38 ]
+adcx r11, rdi
+adc r10, 0x0
+add rbp, r11
+adcx r10, rax
+mulx rax, rdi, r8
+mov r8, rbp
+and r8, r12
+shrd r14, rcx, 52
+shrd rbp, r10, 52
+mov [ r13 + 0x8 ], r8
+xor rcx, rcx
+adox rbp, r9
+adox rbx, rcx
+mulx r11, r9, r14
+adcx rdi, rbp
+adcx rbx, rax
+mov r10, rdi
+shrd r10, rbx, 52
+add r10, [ rsp - 0x18 ]
+add r9, r10
+adc r11, 0x0
+mov rax, r9
+and rax, r12
+and rdi, r12
+shrd r9, r11, 52
+lea r15, [ r15 + r9 ]
+mov [ r13 + 0x20 ], r15
+mov [ r13 + 0x10 ], rdi
+mov [ r13 + 0x18 ], rax
+mov rbx, [ rsp - 0x80 ]
+mov rbp, [ rsp - 0x78 ]
+mov r12, [ rsp - 0x70 ]
+mov r13, [ rsp - 0x68 ]
+mov r14, [ rsp - 0x60 ]
+mov r15, [ rsp - 0x58 ]
+ret
+; cpu AMD Ryzen 7 5800X 8-Core Processor
+; ratio 0.9742
+; seed 3093611607776169 
+; CC / CFLAGS clang / -march=native -mtune=native -O3 
+; time needed: 5798 ms on 1000 evaluations.
+; Time spent for assembling and measuring (initial batch_size=244, initial num_batches=31): 445 ms
+; number of used evaluations: 1000
+; Ratio (time for assembling + measure)/(total runtime for 1000 evals): 0.07675060365643326
+; number reverted permutation / tried permutation: 405 / 496 =81.653%
+; number reverted decision / tried decision: 313 / 503 =62.227%
+; validated in 0.27s
