src/Arithmetic/DettmanMultiplication.v
@@ -15,107 +15,50 @@ Module DettmanMultiplication.
     Context
         (s : Z)
         (c_ : list (Z*Z))
-        (register_width : nat)
         (limbs : nat)
         (weight: nat -> Z)
         (p_nz : s - Associational.eval c_ <> 0)
-        (limbs_gteq_4 : (4 <= limbs)%nat) (* Technically we only need 2 <= limbs to get the proof to go through, but it doesn't make any sense to try to do this with less than three limbs.
-                                           Note that having 4 limbs corresponds to zero iterations of the "loop" function defined below. *)
-        (s_small : forall i: nat, (weight (i + limbs)%nat / weight i) mod s = 0)
+        (limbs_gteq_3 : 3%nat <= limbs) (* Technically we only need 2 <= limbs to get the proof to go through, but it doesn't make any sense to try to do this with less than three limbs.
+                                           Note that having 3 limbs corresponds to zero iterations of the "loop" function defined below. *)
+        (s_small : s <= weight limbs)
         (s_big : weight (limbs - 1)%nat <= s)
-        (weight_lt_width : forall i: nat, (weight i * 2^register_width) mod weight (i + 1)%nat = 0)
+        (weight_limbs_mod_s_eq_0 : (weight limbs) mod s = 0)
         (wprops : @weight_properties weight).
 
-    Context
-        (weight_0 := weight_0 wprops)
-        (weight_positive := weight_positive wprops)
-        (weight_multiples := weight_multiples wprops)
-        (weight_divides := weight_divides wprops).
-    
     Let c := Associational.eval c_.
 
     Lemma s_positive : s > 0.
-    Proof. remember (weight_positive (limbs - 1)). lia. Qed.
+    Proof. remember (weight_positive wprops (limbs - 1)). lia. Qed.
 
     Lemma s_nz : s <> 0.
     Proof. remember s_positive. lia. Qed.
 
     Lemma weight_nz : forall i, weight i <> 0.
-    Proof. intros i. remember (weight_positive i). lia. Qed.
-
-    Lemma div_mul_le : forall x y, y > 0 -> x / y * y <= x.
-    Proof. intros x y H. remember (Zmod_eq x y H). remember (Z_mod_lt x y H). lia. Qed.
+    Proof. intros i. remember (weight_positive wprops i). lia. Qed.
 
     Lemma div_nz a b : b > 0 -> b <= a -> a / b <> 0.
-    Proof. Z.div_mod_to_equations. lia. Qed.
-
-    Lemma weight_div_nz : forall i j : nat, (i <= j)%nat -> weight j / weight i <> 0.
     Proof.
-      intros i j H. assert (0 < weight j / weight i); try lia.
-      apply Weight.weight_divides_full; assumption.
+      intros H1 H2. assert (H: 1 <= a / b).
+      - replace 1 with (b / b).
+        + apply Z_div_le; assumption.
+        + apply Z_div_same. apply H1.
+      - symmetry. apply Z.lt_neq. apply Z.lt_le_trans with 1.
+        + reflexivity.
+        + apply H.
     Qed.
 
-    Lemma s_small' (i j : nat) :
-      (j = i + limbs)%nat ->
-      weight j / weight i mod s = 0.
-    Proof. intros H. subst. apply s_small. Qed.
-
-    Lemma s_big' : s / weight (limbs - 1) <> 0.
-    Proof. remember (weight_positive (limbs - 1)). apply div_nz; lia. Qed.
-
-    Lemma weight_increasing : forall i j : nat, (i <= j)%nat -> weight i <= weight j.
-    Proof.
-      intros i j H.
-      assert (0 < weight j / weight i). { apply Weight.weight_divides_full; try assumption. }
-      assert (1 <= weight j / weight i) by lia.
-      assert (1 * weight i <= weight j / weight i * weight i).
-      { apply Zmult_le_compat_r; try lia. remember (weight_positive i). lia. }
-      apply (Z.le_trans _ (weight j / weight i * weight i) _); try lia.
-      apply div_mul_le. remember (weight_positive i). lia.
-    Qed.
-
-    Lemma mod_quotient_zero : forall x y, 0 < y -> x mod y = 0 -> x mod (x / y) = 0.
-    Proof.
-      intros x y H H1. rewrite Divide.Z.mod_divide_full in H1. destruct H1 as [z H1].
-      subst. rewrite Z_div_mult by lia. rewrite Z.mul_comm. apply Z_mod_mult.
-    Qed.
-    
-    Lemma weight_mod_quotient_zero : forall i j : nat,
-        (i <= j)%nat ->
-        (weight j) mod (weight j / weight i) = 0.
-    Proof.
-      intros i j H. apply mod_quotient_zero; try apply weight_positive.
-      apply Weight.weight_multiples_full; assumption.
-    Qed.
-
-    Lemma divisible_implies_nonzero a b : 
-      a mod b = 0 ->
-      a <> 0 ->
-      a / b <> 0.
-    Proof. intros H1 H2. remember (Z_div_mod_eq_full a b). lia. Qed.
-      
-    Hint Resolve s_positive s_nz weight_nz div_nz s_big' : arith.
+    Hint Resolve s_positive s_nz weight_nz div_nz : arith.
     Hint Resolve weight_0 weight_positive weight_multiples Weight.weight_multiples_full : arith.
-    Hint Resolve weight_div_nz weight_mod_quotient_zero : arith.
-    
+
     Local Open Scope nat_scope.
 
     Definition reduce' x1 x2 x3 x4 x5 := dedup_weights (reduce_one x1 x2 x3 x4 x5).
     Definition carry' x1 x2 x3 := dedup_weights (Associational.carry x1 x2 x3).
 
     Definition loop_body i before :=
-      
-      let from1 := weight (i + limbs) in
-      let to1 := weight (i + limbs + 1) in
-      let middle1 := carry' from1 (to1 / from1) before in
-
-      let from2 := weight (i + limbs) in
-      let to2 := weight i in
-      let middle2 := reduce' s from2 (from2 / to2) c middle1 in
-
-      let from := weight i in
-      let to := weight (i + 1) in
-      let after := carry' from (to / from) middle2 in
+      let middle1 := carry' (weight (i + limbs)) (weight 1) before in
+      let middle2 := reduce' s (weight (i + limbs)) (weight limbs) c middle1 in
+      let after := carry' (weight i) (weight 1) middle2 in
       after.
 
     Hint Rewrite eval_reduce_one Associational.eval_carry eval_dedup_weights: push_eval.
@@ -126,12 +69,12 @@ Module DettmanMultiplication.
     Proof. cbv [loop_body carry' reduce']. autorewrite with push_eval; auto with arith. Qed.
 
     Definition loop start :=
-      fold_right loop_body start (rev (seq 1 (limbs - 2 - 1 - 1))).
+      fold_right loop_body start (rev (seq 1 (limbs - 2 - 1))).
 
     Lemma eval_loop start :
       ((Associational.eval (loop start)) mod (s - c) = (Associational.eval start) mod (s - c))%Z.
     Proof.
-      cbv [loop]. induction (rev (seq 1 (limbs - 2 - 1 - 1))) as [| i l' IHl'].
+      cbv [loop]. induction (rev (seq 1 (limbs - 2 - 1))) as [| i l' IHl'].
       - reflexivity.
       - simpl. rewrite eval_loop_body. apply IHl'.
     Qed.
@@ -139,71 +82,20 @@ Module DettmanMultiplication.
     Definition reduce_carry_borrow r0 :=
       let l := limbs in
       let r0' := dedup_weights r0 in
-      
-      let r1 := carry' (weight (2 * l - 2)) (2^register_width) r0' in
-      
-      let from2 := weight (2 * l - 2) in
-      let to2 := weight (l - 2) in
-      let r2 := reduce' s from2 (from2 / to2) c r1 in
-
-      let from3 := weight (l - 2) in
-      let to3 := weight (l - 1) in
-      let r3 := carry' from3 (to3 / from3) r2 in
-      
-      let from4 := Z.mul (weight (2 * l - 2)) (2^register_width) in
-      let to4 := weight (l - 1) in
-      let r4 := reduce' s from4 (from4 / to4) c r3 in
-
-      let from5 := weight (l - 1) in
-      let to5 := weight l in
-      let r5 := carry' from5 (to5 / from5) r4 in
-
-      let from6 := weight (l - 1) in
-      let to6 := s in
-      let r6 := carry' from6 (to6 / from6) r5 in
-
-      let from7 := weight l in
-      let to7 := weight (l + 1) in
-      let r7 := carry' from7 (to7 / from7) r6 in
-
-      let from8 := weight l in
-      let to8 := s in
-      let r8 := borrow from8 (from8 / to8) r7 in
-      
+      let r1 := carry' (weight (2 * l - 2)) (weight 1) r0' in
+      let r2 := reduce' s (weight (2 * l - 2)) (weight l) c r1 in
+      let r3 := carry' (weight (l - 2)) (weight 1) r2 in
+      let r4 := reduce' s (weight (2 * l - 1)) (weight l) c r3 in
+      let r5 := carry' (weight (l - 1)) (weight 1) r4 in
+      let r6 := carry' (weight (l - 1)) (Z.div s (weight (l - 1))) r5 in
+      let r7 := carry' (weight l) (weight 1) r6 in
+      let r8 := borrow (weight l) (weight l / s) r7 in
       let r8' := dedup_weights r8 in
-      
       let r9 := reduce' s s s c r8' in
-
-      let from10 := weight 0 in
-      let to10 := weight 1 in
-      let r10 := carry' from10 (to10 / from10) r9 in
-      
+      let r10 := carry' (weight 0) (weight 1) r9 in
       let r11 := loop r10 in
-      
-      (* here I've pulled out the final iteration of the loop to do
-         the special register_width carry. *)
-      (* begin final loop iteration *)
-      let i0 := l - 2 - 1 in
-      
-      let rloop1 := carry' (weight (i0 + limbs)) (2^register_width) r11 in
-
-      let fromLoop2 := weight (i0 + limbs) in
-      let toLoop2 := weight i0 in
-      let rloop2 := reduce' s fromLoop2 (fromLoop2 / toLoop2) c rloop1 in
-
-      let fromLoop3 := weight i0 in
-      let toLoop3 := weight (i0 + 1) in
-      let rloop3 := carry' fromLoop3 (toLoop3 / fromLoop3) rloop2 in
-      (* end final loop iteration*)
-      
-      let from12 := Z.mul (weight (i0 + limbs)) (2^register_width) in
-      let to12 := weight (i0 + 1) in
-      let r12 := reduce' s from12 (from12 / to12) c rloop3 in
-
-      let from13 := weight (l - 2) in
-      let to13 := weight (l - 1) in
-      let r13 := carry' from13 (to13 / from13) r12 in
-      
+      let r12 := reduce' s (weight (2 * l - 2)) (weight l) c r11 in
+      let r13 := carry' (weight (l - 2)) (weight 1) r12 in
       Positional.from_associational weight l r13.
 
     Definition mulmod a b :=
@@ -222,62 +114,15 @@ Module DettmanMultiplication.
 
     Local Open Scope Z_scope.
 
-    Lemma reduction_divides i : weight (limbs + i - 1) * 2^register_width / weight i mod s = 0.
-    Proof.
-      rewrite Divide.Z.mod_divide_full. apply (Z.divide_trans _ (weight (limbs + i) / weight i)).
-      - rewrite <- Divide.Z.mod_divide_full. rewrite (Nat.add_comm limbs i). apply s_small.
-      - apply Z.divide_div.
-        + remember (weight_positive i). lia.
-        + rewrite <- Divide.Z.mod_divide_full. apply Weight.weight_multiples_full; try assumption.
-          lia.
-        + rewrite <- Divide.Z.mod_divide_full.
-          replace (weight (limbs + i)) with (weight (limbs + i - 1 + 1)).
-          -- apply weight_lt_width.
-          -- f_equal. lia.
-    Qed.
-
-    Lemma reduction_divides' (i j : nat) :
-      (j = limbs + i - 1)%nat ->
-      weight j * 2^register_width / weight i mod s = 0.
-    Proof. intros H. subst. apply reduction_divides. Qed.
-
-    Lemma weight_prod_mod_zero (i j : nat) :
-      (i <= j)%nat ->
-      (weight j * 2^register_width) mod (weight i) = 0.
-    Proof.
-      intros H. apply Divide.Z.mod_divide_full. apply Z.divide_mul_l.
-      rewrite <- Divide.Z.mod_divide_full. apply Weight.weight_multiples_full; try assumption.
-    Qed.
-    
-    Lemma weight_prod_div_nz (i j : nat) :
-      (i <= j)%nat ->
-      weight j * 2^register_width / weight i <> 0.
-    Proof.
-      intros H. apply divisible_implies_nonzero. apply weight_prod_mod_zero; try lia.
-      remember (weight_positive j). remember (Z.pow_nonneg 2 register_width). lia.
-    Qed.
-
-    Lemma s_small_particular : weight limbs mod s = 0.
-    Proof.
-      replace (weight limbs) with (weight limbs / weight 0).
-      - apply s_small'; lia.
-      - Z.div_mod_to_equations. lia.
-    Qed.
-      
     Lemma eval_reduce_carry_borrow r0 :
       (Positional.eval weight limbs (reduce_carry_borrow r0)) mod (s - c) =
       (Associational.eval r0) mod (s - c).
     Proof.
       cbv [reduce_carry_borrow carry' reduce']. autorewrite with push_eval; auto with arith.
-      all: try apply weight_div_nz; try lia.
-      all: try apply weight_mod_quotient_zero; try lia.
-      all: try apply reduction_divides'; try lia.
-      all: try apply weight_prod_div_nz; try lia.
-      all: try apply s_small'; try lia.
-      all: try apply mod_quotient_zero; try apply divisible_implies_nonzero; try apply s_small_particular; try apply weight_positive.
-      all: try apply weight_prod_mod_zero; try lia.
-      all: try (remember (weight_positive limbs); lia).
-      all: try (remember s_positive; lia).
+      all: try apply Weight.weight_multiples_full; auto with arith; try lia.
+      - apply div_nz; try assumption. remember (weight_positive wprops (limbs - 1)). lia.
+      - apply Divide.Z.mod_divide_full in weight_limbs_mod_s_eq_0. destruct weight_limbs_mod_s_eq_0 as [x H].
+        rewrite H. rewrite Z_div_mult; try apply s_positive. rewrite Z.mul_comm. rewrite Z_mod_mult. lia.
     Qed.
 
     Hint Rewrite eval_reduce_carry_borrow : push_eval.
@@ -307,33 +152,23 @@ Module dettman_multiplication_mod_ops.
     Context
         (s : Z)
         (c : list (Z*Z))
-        (register_width : nat)
         (n : nat)
         (last_limb_width : nat)
         (p_nz : s - Associational.eval c <> 0)
-        (n_gteq_4 : (4 <= n)%nat)
-        (last_limb_width_small : last_limb_width * n <= Z.log2 s)
+        (n_gteq_3 : 3%nat <= n)
+        (last_limb_width_small : last_limb_width * n <= Z.log2_up s)
         (last_limb_width_big : 1 <= last_limb_width)
         (s_power_of_2 : 2 ^ (Z.log2 s) = s).
 
-    (* I do want to have Z.log2 s, not Z.log2_up (s - c) below.  We want to ensure that weight (n - 1) <= s <= weight limbs *)
-    Local Notation limbwidth_num' := (Z.log2 s - last_limb_width).
-    Local Notation limbwidth_den' := (n - 1). (* can't use Q here, or else reification doesn't work *)
-    
-    Context
-        (registers_big : limbwidth_num' <= register_width * limbwidth_den') (* stated somewhat awkwardly in terms of Z; i think we might want to avoid Q here too *)
-        (weight_big : Z.log2 s <= n * limbwidth_num' / limbwidth_den').
-
-    (* I don't want these to be automatically unfolded in the proofs below. *)
-    Definition limbwidth_num := limbwidth_num'.
-    Definition limbwidth_den := limbwidth_den'.
-    
+    (* I do want to have Z.log2_up s, not Z.log2_up (s - c) below.  We want to ensure that weight (n - 1) <= s <= weight limbs *)
+    Local Notation limbwidth_num := (Z.log2_up s - last_limb_width).
+    Local Notation limbwidth_den := (n - 1). (* can't use Q here, or else reification doesn't work *)
     Definition weight := (weight limbwidth_num limbwidth_den).
     
-    Definition mulmod := mulmod s c register_width n weight.
-    Definition squaremod := squaremod s c register_width n weight.
+    Definition mulmod := mulmod s c n weight.
+    Definition squaremod := squaremod s c n weight.
 
-    Lemma n_small : n - 1 <= Z.log2 s - last_limb_width.
+    Lemma n_small : n - 1 <= Z.log2_up s - last_limb_width.
     Proof.
       replace (Z.of_nat n) with (Z.of_nat n - 1 + 1) in last_limb_width_small by lia.
       remember (Z.of_nat n - 1) as n'.
@@ -346,123 +181,69 @@ Module dettman_multiplication_mod_ops.
     Qed.
 
     Lemma limbwidth_good : 0 < limbwidth_den <= limbwidth_num.
-    Proof. remember n_small. cbv [limbwidth_den limbwidth_num]. lia. Qed.
+    Proof. remember n_small. lia. Qed.
 
     Local Notation wprops := (@wprops limbwidth_num limbwidth_den limbwidth_good).
 
-    Lemma Qceiling_diff x y : Qfloor (x - y) <= Qceiling x - Qceiling y.
+    Lemma s_small : s <= weight n.
     Proof.
-      assert (H: Qfloor (x - y) + Qceiling y <= Qceiling x).
-      - replace (Qceiling x) with (Qceiling (x - y + y))%Q.
-        + apply QUtil.add_floor_l_le_ceiling.
-        + cbv [Qminus].
-          rewrite <- Qplus_assoc. rewrite (Qplus_comm (-y) y).
-          rewrite Qplus_opp_r. rewrite Qplus_0_r. reflexivity.
-      - lia.
+      rewrite (ModOps.weight_ZQ_correct _ _ limbwidth_good).
+      remember (Log2.Z.log2_up_le_full s) as H eqn:clearMe. clear clearMe.
+      apply (Z.le_trans _ _ _ H). apply Z.pow_le_mono_r; try lia.
+      rewrite Zle_Qle.
+      remember (_ *_)%Q as x eqn:E. apply (Qle_trans _ x).
+      - subst. rewrite <- (Qmult_le_r _ _ (inject_Z (Z.of_nat n) - 1)).
+        + cbv [Qdiv Qminus]. replace 0%Q with (inject_Z 0) by reflexivity.
+          replace (-(1))%Q with (inject_Z (-1)) by reflexivity. rewrite <- inject_Z_plus.
+          rewrite <- inject_Z_mult. repeat rewrite <- Qmult_assoc. rewrite (Qmult_comm (Qinv _)).
+          rewrite <- (Qmult_assoc _ _ (Qinv _)). rewrite Qmult_inv_r.
+          -- rewrite Qmult_1_r. rewrite <- inject_Z_mult. rewrite <- Zle_Qle. lia.
+          -- replace 0%Q with (inject_Z 0) by reflexivity. rewrite inject_Z_injective. lia.
+        + replace 0%Q with (inject_Z 0) by reflexivity.
+          replace 1%Q with (inject_Z 1) by reflexivity. cbv [Qminus]. rewrite <- inject_Z_opp.
+          rewrite <- inject_Z_plus. rewrite <- Zlt_Qlt. lia.
+      - apply Qle_ceiling.
     Qed.
 
-    Lemma Qopp_distr_mul_r x y : (- (x * y) == x * -y)%Q.
-    Proof. cbv [Qmult Qopp Qeq]. simpl. lia. Qed.      
-      
-    Lemma s_small : forall i : nat, (weight (i + n) / weight i) mod s = 0.
-    Proof.
-      intros i. repeat rewrite (ModOps.weight_ZQ_correct _ _ limbwidth_good).
-      rewrite <- Z.pow_sub_r; try lia.
-      - rewrite <- s_power_of_2. apply Modulo.Z.mod_same_pow. split.
-        + apply Z.log2_nonneg.
-        + remember (_ * (i + n)%nat)%Q as x. remember (_ * i)%Q as y.
-          apply (Z.le_trans _ (Qfloor (x - y))).
-          -- subst. cbv [Qminus]. rewrite Qopp_distr_mul_r. rewrite <- Qmult_plus_distr_r.
-             rewrite <- inject_Z_opp. rewrite <- inject_Z_plus.
-             replace (Z.of_nat (i + n) + - Z.of_nat i) with (Z.of_nat n) by lia.
-             replace (Z.log2 s) with (Qfloor (inject_Z (Z.log2 s))).
-             ++ apply Qfloor_resp_le. rewrite Qmult_comm.
-                apply (Qle_trans _ (inject_Z (n * limbwidth_num / limbwidth_den)))%Z.
-                --- rewrite <- Zle_Qle. apply weight_big.
-                --- cbv [Qdiv]. rewrite Zdiv_Qdiv.
-                    apply (Qle_trans _ ((n * limbwidth_num)%Z / limbwidth_den)).
-                    +++ apply Qfloor_le.
-                    +++ rewrite inject_Z_mult. rewrite Qmult_assoc. apply Qle_refl.
-             ++ apply Qfloor_Z.
-          -- apply Qceiling_diff.
-      - remember limbwidth_good as H eqn:clearMe; clear clearMe. split.
-        + replace 0 with (Qceiling 0) by reflexivity. apply Qceiling_resp_le.
-          apply Qmult_le_0_compat.
-          -- cbv [Qdiv]. apply Qmult_le_0_compat.
-             ++ replace 0%Q with (inject_Z 0) by reflexivity. rewrite <- Zle_Qle. lia.
-             ++ apply Qinv_le_0_compat. replace 0%Q with (inject_Z 0) by reflexivity.
-                rewrite <- Zle_Qle. lia.
-          -- replace 0%Q with (inject_Z 0) by reflexivity. rewrite <- Zle_Qle. lia.
-        + apply Qceiling_resp_le. rewrite Qmult_comm. rewrite (Qmult_comm (_ / _)).
-          apply Qmult_le_compat_r.
-          -- rewrite <- Zle_Qle. lia.
-          -- cbv [Qdiv]. apply Qmult_le_0_compat.
-             ++ replace 0%Q with (inject_Z 0) by reflexivity. rewrite <- Zle_Qle. lia.
-             ++ apply Qinv_le_0_compat. replace 0%Q with (inject_Z 0) by reflexivity.
-                rewrite <- Zle_Qle. lia.
-    Qed.
-      
     Lemma s_gt_0 : 0 < s.
       assert (H: s <= 0 \/ 0 < s) by lia. destruct H as [H|H].
-      - apply Z.log2_nonpos in H. lia.
+      - apply Z.log2_up_nonpos in H. lia.
       - assumption.
     Qed.
 
     Lemma s_big : weight (n - 1) <= s.
     Proof.
       rewrite (ModOps.weight_ZQ_correct _ _ limbwidth_good).
-      cbv [limbwidth_num limbwidth_den]. 
       remember (Z.log2_spec _ s_gt_0) as H eqn:clearMe. clear clearMe.
       destruct H as [H _].
       apply (Z.le_trans _ (2 ^ Z.log2 s)); try apply H.
       apply Z.pow_le_mono_r; try lia.
       rewrite Zle_Qle. cbv [Qdiv]. rewrite <- (Qmult_assoc _ (Qinv _)).
       rewrite (Qmult_comm (Qinv _)). rewrite Nat2Z.inj_sub; try lia. simpl. cbv [Z.sub].
-      rewrite inject_Z_plus. simpl. cbv [Qminus]. rewrite Qmult_inv_r.
+      rewrite inject_Z_plus. simpl. replace (inject_Z (-1)) with (-(1))%Q by reflexivity.
+      cbv [Qminus]. rewrite Qmult_inv_r.
       - rewrite <- inject_Z_plus. rewrite Qmult_1_r. rewrite Qceiling_Z.
         rewrite <- Zle_Qle. remember (Z.le_log2_up_succ_log2 s). lia.
-      - replace 0%Q with (inject_Z 0) by reflexivity. rewrite inject_Z_injective. lia.
+      - replace (-(1))%Q with (inject_Z (-1)) by reflexivity.
+        replace 0%Q with (inject_Z 0) by reflexivity. rewrite inject_Z_injective. lia.
     Qed.
 
-    Lemma weight_lt_width : forall i: nat, (weight i * 2^register_width) mod weight (i + 1)%nat = 0.
+    Lemma weight_n_mod_s_eq_0 : weight n mod s = 0.
     Proof.
-      intros i. repeat rewrite (ModOps.weight_ZQ_correct _ _ limbwidth_good).
-      remember limbwidth_good eqn:clearMe; clear clearMe.
-      rewrite <- Z.pow_add_r; try lia.
-      - apply Modulo.Z.mod_same_pow. split.
-        + remember (_ / _ * _)%Q as x. replace 0 with (Qceiling 0%Z) by reflexivity.
-          apply Qceiling_resp_le. subst. replace (inject_Z 0) with 0%Q by reflexivity.
-          cbv [Qdiv]. apply Qmult_le_0_compat.
-          -- apply Qmult_le_0_compat.
-             ++ replace 0%Q with (inject_Z 0) by reflexivity. rewrite <- Zle_Qle. lia.
-             ++ apply Qinv_le_0_compat. replace 0%Q with (inject_Z 0) by reflexivity.
-                rewrite <- Zle_Qle. lia.
-          -- replace 0%Q with (inject_Z 0) by reflexivity. rewrite <- Zle_Qle. lia.
-        + rewrite Nat2Z.inj_add. rewrite inject_Z_plus. rewrite Qmult_plus_distr_r.
-          remember (_ / _ * i)%Q as x. remember (_ / _ * 1%nat)%Q as y.
-          apply (Z.le_trans _ (Qceiling x + Qceiling y)).
-          -- apply QUtil.Qceiling_le_add.
-          -- assert (Qceiling y <= register_width); try lia.
-             replace (Z.of_nat register_width) with (Qceiling (inject_Z register_width)).
-             ++ apply Qceiling_resp_le. subst.
-                replace (inject_Z (Z.of_nat 1)) with 1%Q by reflexivity.
-                rewrite Qmult_1_r. apply Qle_shift_div_r.
-                --- remember limbwidth_good. replace 0%Q with (inject_Z 0) by reflexivity.
-                    rewrite <- Zlt_Qlt. lia.
-                --- rewrite <- inject_Z_mult. rewrite <- Zle_Qle.
-                    cbv [limbwidth_num limbwidth_den]. lia.
-             ++ apply Qceiling_Z.
-      - replace 0 with (Qceiling 0) by reflexivity. apply Qceiling_resp_le.
-        apply Qmult_le_0_compat.
-        + cbv [Qdiv]. apply Qmult_le_0_compat.
-          -- replace 0%Q with (inject_Z 0) by reflexivity. rewrite <- Zle_Qle. lia.
-          -- apply Qinv_le_0_compat. replace 0%Q with (inject_Z 0) by reflexivity.
-             rewrite <- Zle_Qle. lia.
-        + replace 0%Q with (inject_Z 0) by reflexivity. rewrite <- Zle_Qle. lia.
+      cbv [weight ModOps.weight]. remember (- _) as e eqn:E. rewrite <- s_power_of_2.
+      apply Modulo.Z.mod_same_pow. split.
+      - apply Z.log2_nonneg.
+      - assert (H: 0 < 2) by lia. rewrite (Z.pow_le_mono_r_iff 2); try lia.
+        + subst. replace (2^(-_)) with (weight n) by reflexivity. rewrite s_power_of_2.
+          apply s_small.
+        + remember (weight_positive wprops n) as H1 eqn:clearMe. clear clearMe.
+          cbv [ModOps.weight] in H1. rewrite <- E in H1.
+          assert (H': 0 <= e \/ e < 0) by lia. destruct H' as [H'|H']; try lia.
+          apply (Z.pow_neg_r 2 _) in H'. lia.
     Qed.
-
-    Definition eval_mulmod := eval_mulmod s c register_width n weight p_nz n_gteq_4 s_small s_big weight_lt_width wprops.
-    Definition eval_squaremod := eval_squaremod s c register_width n weight p_nz n_gteq_4 s_small s_big weight_lt_width wprops.
+ 
+    Definition eval_mulmod := eval_mulmod s c n weight p_nz n_gteq_3 s_small s_big weight_n_mod_s_eq_0 wprops.
+    Definition eval_squaremod := eval_squaremod s c n weight p_nz n_gteq_3 s_small s_big weight_n_mod_s_eq_0 wprops.
   End dettman_multiplication_mod_ops.
 End dettman_multiplication_mod_ops.
 
